string cancellation done! (except for the actual simproc)

src/Lean/Meta/Tactic/Simp/BuiltinSimprocs/StringEq.lean
@@ -8,29 +8,57 @@ module
 prelude
 public import Lean.Meta.Tactic.Simp.BuiltinSimprocs.Char
 import Init.Data.String.SimpEq
-import Lean.Meta.StringLitProof
+import Init.Data.String.Lemmas.FindPos
+import Init.While
+public meta import Lean.Elab.Command
+
+meta section
 
 namespace String
 
 open Lean Meta
 open Internal.SimpEq
 
-inductive ExprStructure where
-  -- String
-  | stringAppend (a b : ExprStructure)
-  | push (s : ExprStructure) (c : Expr)
-  | singleton (c : Expr)
-  | ofList (l : ExprStructure)
-  | stringLit (s : String)
-  | anyString (s : Expr)
-  -- List Char
-  | nil
-  | cons (c : Expr) (l : ExprStructure)
-  | listAppend (a b : ExprStructure)
-  | toList (s : ExprStructure)
-  | anyList (l : Expr)
+inductive ExprType where
+  | string
+  | list
+  | char
+deriving DecidableEq, Repr
 
-def ExprStructure.maxDepth : ExprStructure → Nat
+deriving instance Repr for String.Pos
+deriving instance Repr for Slice
+
+-- Regarding erased parts: erased parts indicate what has been cancelled out in the
+-- `cancelLeft` / `cancelRight` procedures; we treat the like `anyXYZ` but don't allow them
+-- to be cancelled again (see `isDefEq` / `isCompatibleWith`)
+inductive ExprStructure : ExprType → Type where
+  -- String
+  | stringAppend (a b : ExprStructure .string) : ExprStructure .string
+  | push (s : ExprStructure .string) (c : ExprStructure .char) : ExprStructure .string
+  | singleton (c : ExprStructure .char) : ExprStructure .string
+  | ofList (l : ExprStructure .list) : ExprStructure .string
+  /--
+  `s.str.sliceTo s.startInclusive` and `s.str.sliceFrom s.endExclusive` are erased but still part
+  of the original expression
+  -/
+  | stringLit (s : String.Slice) : ExprStructure .string
+  | anyString (s : Expr) : ExprStructure .string
+  | erasedString (s : Expr) : ExprStructure .string
+  -- List Char
+  | nil : ExprStructure .list
+  | cons (c : ExprStructure .char) (l : ExprStructure .list) : ExprStructure .list
+  | listAppend (a b : ExprStructure .list) : ExprStructure .list
+  | toList (s : ExprStructure .string) : ExprStructure .list
+  | anyList (l : Expr) : ExprStructure .list
+  | erasedList (l : Expr) : ExprStructure .list
+  -- Char
+  | charLit (c : Char) : ExprStructure .char
+  | anyChar (c : Expr) : ExprStructure .char
+  | erasedChar (c : Expr) : ExprStructure .char
+deriving Repr
+
+-- TODO: make this a computed field (private inductives can't have computed fields???)
+def ExprStructure.maxDepth : ExprStructure ty → Nat
   -- String
   | .stringAppend a b => max a.maxDepth b.maxDepth + 1
   | .push s _ => s.maxDepth + 1
@@ -38,98 +66,61 @@ def ExprStructure.maxDepth : ExprStructure → Nat
   | .ofList l => l.maxDepth + 1
   | .stringLit _ => 0
   | .anyString _ => 0
+  | .erasedString _ => 0
   -- List Char
   | .nil => 0
   | .cons _ l => l.maxDepth + 1
   | .listAppend a b => max a.maxDepth b.maxDepth + 1
   | .toList s => s.maxDepth + 1
   | .anyList _ => 0
+  | .erasedList _ => 0
+  -- Char
+  | .charLit _ => 0
+  | .anyChar _ => 0
+  | .erasedChar _ => 0
 
-protected def ExprStructure.isDefEq : ExprStructure → ExprStructure → MetaM Bool
-  | .stringAppend a b, .stringAppend a' b' => a.isDefEq a' <&&> b.isDefEq b'
-  | .push s c, .push s' c' => s.isDefEq s' <&&> isDefEq c c'
-  | .singleton c, .singleton c' => isDefEq c c'
-  | .ofList l, .ofList l' => l.isDefEq l'
-  | .stringLit s, .stringLit s' => pure (s == s')
-  | .anyString s, .anyString s' => isDefEq s s'
-  | .nil, .nil => pure true
-  | .cons c l, .cons c' l' => isDefEq c c' <&&> l.isDefEq l'
-  | .listAppend a b, .listAppend a' b' => a.isDefEq a' <&&> b.isDefEq b'
-  | .toList s, .toList s' => s.isDefEq s'
-  | .anyList l, .anyList l' => isDefEq l l'
-  | _, _ => pure false
-
-inductive CancelElement where
-  | cons (l r : Expr)
-  | string (e : Expr)
-  | list (e : Expr)
-  | char (e : Expr)
-
-inductive Path where
-  | root
+-- TODO: make this a computed field (private inductives can't have computed fields???)
+def ExprStructure.isEmpty : ExprStructure ty → Bool
   -- String
-  | stringAppendLeft (parent : Path) (right : ExprStructure)
-  | stringAppendRight (parent : Path) (left : ExprStructure)
-  | push (parent : Path) (c : Expr)
-  | toList (parent : Path)
+  | .stringAppend a b => a.isEmpty && b.isEmpty
+  | .push _ _ => false
+  | .singleton _ => false
+  | .ofList l => l.isEmpty
+  | .stringLit s => s.str.isEmpty
+  | .anyString _ => false
+  | .erasedString _=> false
   -- List Char
-  | cons (parent : Path) (c : Expr)
-  | listAppendLeft (parent : Path) (right : ExprStructure)
-  | listAppendRight (parent : Path) (left : ExprStructure)
-  | ofList (parent : Path)
-
-def Path.innerLeft : Path → ExprStructure → Option (Path × ExprStructure)
-  | p, .stringAppend l r => some (.stringAppendLeft p r, l)
-  | p, .push s c => some (.push p c, s)
-  | p, .ofList l => some (.ofList p, l)
-  | _, .singleton _ | _, .stringLit _ | _, .anyString _ => none
-  -- List Char
-  | _, .nil | _, .cons .. => none
-  | p, .listAppend l r => some (.listAppendLeft p r, l)
-  | p, .toList s => some (.toList p, s)
-  | _, .anyList _ => none
-
-def Path.next : Path → ExprStructure → Path × ExprStructure
-  | .root, e => (.root, e)
-  -- String
-  | .stringAppendLeft parent right, left => (.stringAppendRight parent left, right)
-  | .stringAppendRight parent left, right => parent.next (.stringAppend left right)
-  | .push parent c, s => parent.next (.push s c)
-  | .toList parent, s => parent.next (.toList s)
-  -- List Char
-  | .cons parent c, s => parent.next (.cons c s)
-  | .listAppendLeft parent right, left => (.listAppendRight parent left, right)
-  | .listAppendRight parent left, right => parent.next (.listAppend left right)
-  | .ofList parent, l => parent.next (.ofList l)
-
-def Path.toStruct : Path → ExprStructure → ExprStructure
-  | .root, e => e
-  -- String
-  | .stringAppendLeft parent right, left => parent.toStruct (.stringAppend left right)
-  | .stringAppendRight parent left, right => parent.toStruct (.stringAppend left right)
-  | .push parent c, s => parent.toStruct (.push s c)
-  | .toList parent, s => parent.toStruct (.toList s)
-  -- List Char
-  | .cons parent c, s => parent.toStruct (.cons c s)
-  | .listAppendLeft parent right, left => parent.toStruct (.listAppend left right)
-  | .listAppendRight parent left, right => parent.toStruct (.listAppend left right)
-  | .ofList parent, l => parent.toStruct (.ofList l)
+  | .nil => true
+  | .cons _ _ => false
+  | .listAppend a b => a.isEmpty && b.isEmpty
+  | .toList s => s.isEmpty
+  | .anyList _ => false
+  | .erasedList _=> false
+  -- Char
+  | .charLit _ => false
+  | .anyChar _ => false
+  | .erasedChar _=> false
 
 def listAppendInst : Expr :=
-  mkApp2 (.const ``instHAppendOfAppend [0, 0, 0]) (.app (mkConst ``List) (mkConst ``Char))
+  mkApp2 (.const ``instHAppendOfAppend [0]) (.app (mkConst ``List) (mkConst ``Char))
     (.app (.const ``List.instAppend [0]) (mkConst ``Char))
 
 def stringAppendInst : Expr :=
-  mkApp2 (.const ``instHAppendOfAppend [0, 0, 0]) (mkConst ``String) (mkConst ``instAppendString)
+  mkApp2 (.const ``instHAppendOfAppend [0]) (mkConst ``String) (mkConst ``instAppendString)
+
+@[match_pattern]
+def mkCharLit (n : Nat) : Expr :=
+  .app (.const ``Char.ofNat []) (mkRawNatLit n)
 
 mutual
 
-partial def createStringStructure (e : Expr) : MetaM ExprStructure := do
-  if let mkStrLit s := e then
+partial def createStringStructure (e : Expr) : MetaM (ExprStructure .string) := do
+  let e' ← whnf e
+  if let mkStrLit s := e' then
     return .stringLit s
-  match_expr e with
-  | String.push s c => return .push (← createStringStructure s) c
-  | String.singleton c => return .singleton c
+  match_expr e' with
+  | String.push s c => return .push (← createStringStructure s) (← createCharStructure c)
+  | String.singleton c => return .singleton (← createCharStructure c)
   | String.ofList l => return .ofList (← createListStructure l)
   | HAppend.hAppend _ _ _ inst a b =>
     if ← pure (inst == stringAppendInst) <||> isDefEqI inst stringAppendInst then
@@ -137,10 +128,11 @@ partial def createStringStructure (e : Expr) : MetaM ExprStructure := do
     return .anyString e
   | _ => return .anyString e
 
-partial def createListStructure (e : Expr) : MetaM ExprStructure := do
-  match_expr e with
-  | List.nil => return .nil
-  | List.cons c l => return .cons c (← createListStructure l)
+partial def createListStructure (e : Expr) : MetaM (ExprStructure .list) := do
+  let e' ← whnf e
+  match_expr e' with
+  | List.nil _ => return .nil
+  | List.cons _ c l => return .cons (← createCharStructure c) (← createListStructure l)
   | String.toList s => return .toList (← createStringStructure s)
   | HAppend.hAppend _ _ _ inst a b =>
     if ← pure (inst == listAppendInst) <||> isDefEqI inst listAppendInst then
@@ -148,7 +140,755 @@ partial def createListStructure (e : Expr) : MetaM ExprStructure := do
     return .anyList e
   | _ => return .anyList e
 
+partial def createCharStructure (e : Expr) : MetaM (ExprStructure .char) := do
+  let e' ← whnf e
+  match e' with
+  | mkCharLit n => return .charLit (Char.ofNat n)
+  | _ => return .anyChar e
+
 end
+
+protected def ExprStructure.toExpr : ExprStructure ty → Expr
+  -- String
+  | .stringAppend a b =>
+    let stringAppend := mkApp4 (.const ``HAppend.hAppend [0, 0, 0])
+      (mkConst ``String) (mkConst ``String) (mkConst ``String) stringAppendInst
+    mkApp2 stringAppend a.toExpr b.toExpr
+  | .push s c => mkApp2 (mkConst ``String.push) s.toExpr c.toExpr
+  | .singleton c => .app (mkConst ``String.singleton) c.toExpr
+  | .ofList l => .app (mkConst ``String.ofList) l.toExpr
+  | .stringLit s => mkStrLit s.str
+  | .anyString s => s
+  | .erasedString s => s
+  -- List Char
+  | .nil => .app (.const ``List.nil [0]) (mkConst ``Char)
+  | .cons c l =>
+    let cons := .app (.const ``List.cons [0]) (mkConst ``Char)
+    mkApp2 cons c.toExpr l.toExpr
+  | .listAppend a b =>
+    let listAppend :=  mkApp4 (.const ``HAppend.hAppend [0, 0, 0])
+      (.app (mkConst ``List) (mkConst ``Char)) (.app (mkConst ``List) (mkConst ``Char))
+      (.app (mkConst ``List) (mkConst ``Char)) listAppendInst
+    mkApp2 listAppend a.toExpr b.toExpr
+  | .toList s => .app (mkConst ``String.toList) s.toExpr
+  | .anyList l => l
+  | .erasedList l => l
+  -- Char
+  | .charLit c => mkCharLit c.toNat
+  | .anyChar c => c
+  | .erasedChar c => c
+
+protected def ExprStructure.toStructExpr : ExprStructure ty → Expr
+  -- String
+  | .stringAppend a b => mkApp2 (mkConst ``StringStructure.append) a.toStructExpr b.toStructExpr
+  | .push s c => mkApp2 (mkConst ``StringStructure.push) s.toStructExpr c.toStructExpr
+  | .singleton c => .app (mkConst ``StringStructure.singleton) c.toStructExpr
+  | .ofList l => .app (mkConst ``StringStructure.ofList) l.toStructExpr
+  | .stringLit s => .app (mkConst ``StringStructure.lit) (ToExpr.toExpr s.str.toList)
+  | .anyString s => .app (mkConst ``StringStructure.any) s
+  | .erasedString s => .app (mkConst ``StringStructure.any) s
+  -- List Char
+  | .nil => mkConst ``ListStructure.nil
+  | .cons c l => mkApp2 (mkConst ``ListStructure.cons) c.toStructExpr l.toStructExpr
+  | .listAppend a b => mkApp2 (mkConst ``ListStructure.append) a.toStructExpr b.toStructExpr
+  | .toList s => .app (mkConst ``ListStructure.toList) s.toStructExpr
+  | .anyList l => .app (mkConst ``ListStructure.any) l
+  | .erasedList l => .app (mkConst ``ListStructure.any) l
+  -- Char
+  | .charLit c => mkCharLit c.toNat
+  | .anyChar c => c
+  | .erasedChar c => c
+
+/--
+Returns true iff both structures are definitionally equivalent and don't contain any erased parts.
+-/
+protected def ExprStructure.isDefEq : ExprStructure ty → ExprStructure ty → MetaM Bool
+  -- String
+  | .stringAppend a b, .stringAppend a' b' => a.isDefEq a' <&&> b.isDefEq b'
+  | .push s c, .push s' c' => s.isDefEq s' <&&> c.isDefEq c'
+  | .singleton c, .singleton c' => c.isDefEq c'
+  | .ofList l, .ofList l' => l.isDefEq l'
+  | .stringLit s, .stringLit s' => pure (s == s')
+  | .anyString s, .anyString s' => isDefEq s s'
+  -- List Char
+  | .nil, .nil => pure true
+  | .cons c l, .cons c' l' => c.isDefEq c' <&&> l.isDefEq l'
+  | .listAppend a b, .listAppend a' b' => a.isDefEq a' <&&> b.isDefEq b'
+  | .toList s, .toList s' => s.isDefEq s'
+  | .anyList l, .anyList l' => isDefEq l l'
+  -- Char
+  | .charLit c, .charLit c' => pure (c == c')
+  | .anyChar c, .anyChar c' => isDefEq c c'
+  -- We don't want to erase any already erased parts
+  -- and thus make `isDefEq` irreflexive for `erasedString` / `erasedList` / `erasedChar`
+  | _, _ => pure false
+
+/--
+Returns true iff both structures are definitionally equivalent or both characters and don't contain
+any erased parts.
+-/
+protected def ExprStructure.isCompatibleWith
+    (a : ExprStructure ty) (b : ExprStructure ty') : MetaM (Option (PLift (ty = ty'))) := do
+  if h : ty = ty' then
+    if ty matches .char then
+      if a matches .erasedChar _ || b matches .erasedChar _ then
+        pure none
+      else
+        pure (some ⟨h⟩)
+    else if ← a.isDefEq (h ▸ b) then
+      pure (some ⟨h⟩)
+    else
+      pure none
+  else pure none
+
+def ExprStructure.toAny (x : ExprStructure ty) : ExprStructure ty :=
+  match ty with
+  | .string => .anyString x.toExpr
+  | .list => .anyList x.toExpr
+  | .char => .anyChar x.toExpr
+
+inductive ErasureResult (ty : ExprType) where
+  | empty
+  | noErased
+  | result (x : ExprStructure ty)
+
+@[inline]
+def ErasureResult.valueD (x : ErasureResult ty) (default : ExprStructure ty) :
+    ExprStructure ty :=
+  match x with
+  | .result x => x
+  | _ => default
+
+@[inline]
+def ErasureResult.elim (x : ErasureResult ty) (empty noErased : ExprStructure ty) :
+    ExprStructure ty :=
+  match x with
+  | .empty => empty
+  | .noErased => noErased
+  | .result x => x
+
+@[inline]
+def ErasureResult.withErased (x : ErasureResult ty) (val : ExprStructure ty) :
+    ErasureResult ty :=
+  match x with
+  | .noErased => .result val.toAny
+  | x => x
+
+@[inline]
+def ErasureResult.map (f : ExprStructure ty → ExprStructure ty') :
+    ErasureResult ty → ErasureResult ty'
+  | .empty => .empty
+  | .noErased => .noErased
+  | .result x => .result (f x)
+
+def ExprStructure.removeErased : ExprStructure ty → ErasureResult ty
+  -- String
+  | .stringAppend a b =>
+    match a.removeErased, b.removeErased with
+    | .empty, res => res.withErased b
+    | res, .empty => res.withErased a
+    | .noErased, .noErased => .noErased
+    | res, res' => .result (.stringAppend (res.valueD a) (res'.valueD b))
+  | .push s c =>
+    match s.removeErased, c.removeErased with
+    | .empty, .empty => .empty
+    | .empty, res => (res.withErased c).map .singleton
+    | res, .empty => res.withErased s
+    | .noErased, .noErased => .noErased
+    | res, res' => .result (.push (res.valueD s) (res'.valueD c))
+  | .singleton c => c.removeErased.map .singleton
+  | .ofList l => l.removeErased.map .ofList
+  | .stringLit s =>
+    if s.startInclusive = s.str.startPos ∧ s.endExclusive = s.str.endPos then
+      .noErased
+    else if s.isEmpty then
+      .empty
+    else
+      .result (.stringLit s.copy)
+  | .anyString _ => .noErased
+  | .erasedString _ => .empty
+  -- List Char
+  | .nil => .noErased
+  | .cons c l =>
+    match c.removeErased, l.removeErased with
+    | .empty, res => if l matches .nil then .empty else res.withErased l
+    | .noErased, .empty | .result c, .empty => .result (.cons c .nil)
+    | .noErased, .noErased => .noErased
+    | res, res' => .result (.cons (res.valueD c) (res'.valueD l))
+  | .listAppend a b =>
+    match a.removeErased, b.removeErased with
+    | .empty, res => res.withErased b
+    | res, .empty => res.withErased a
+    | .noErased, .noErased => .noErased
+    | res, res' => .result (.listAppend (res.valueD a) (res'.valueD b))
+  | .toList l => l.removeErased.map .toList
+  | .anyList _ => .noErased
+  | .erasedList _ => .empty
+  -- Char
+  | .charLit _ => .noErased
+  | .anyChar _ => .noErased
+  | .erasedChar _ => .empty
+
+def ExprStructure.removeErasedTop (e : ExprStructure .string) : ExprStructure .string :=
+  match e.removeErased with
+  | .empty => .stringLit ""
+  | .noErased => e.toAny
+  | .result x => x
+
+inductive CancelElement where
+  | cons (l r : Expr)
+  | string (e : Expr)
+  | list (e : Expr)
+  | char (e : Expr)
+deriving Repr
+
+def cancelElementToStruct (as : Array CancelElement) : Expr :=
+  as.foldr (init := mkConst ``Cancellation.nil) fun
+    | .cons l r, s => mkApp3 (mkConst ``Cancellation.cons) l r s
+    | .string e, s => mkApp2 (mkConst ``Cancellation.string) e s
+    | .list e, s => mkApp2 (mkConst ``Cancellation.list) e s
+    | .char e, s => mkApp2 (mkConst ``Cancellation.char) e s
+
+inductive Element where
+  | string (e : Expr)
+  | list (e : Expr)
+  | char (e : Expr)
+
+def CancelElement.left : CancelElement → Element
+  | .cons l _ => .char l
+  | .string e => .string e
+  | .list e => .list e
+  | .char e => .char e
+
+def CancelElement.right : CancelElement → Element
+  | .cons _ r => .char r
+  | .string e => .string e
+  | .list e => .list e
+  | .char e => .char e
+
+def ExprStructure.elements : ExprStructure ty → List Element
+  -- String
+  | .stringAppend a b => a.elements ++ b.elements
+  | .push s c => s.elements ++ c.elements
+  | .singleton c => c.elements
+  | .ofList l => l.elements
+  | .stringLit s => s.str.toList.map (fun c => .char (mkCharLit c.toNat))
+  | .anyString s | .erasedString s => [.string s]
+  -- List Char
+  | .nil => []
+  | .cons c l => c.elements ++ l.elements
+  | .listAppend a b => a.elements ++ b.elements
+  | .toList s => s.elements
+  | .anyList l | .erasedList l => [.list l]
+  -- Char
+  | .charLit c => [.char (mkCharLit c.toNat)]
+  | .anyChar c | .erasedChar c => [.char c]
+
+@[local simp]
+theorem ExprStructure.elements_char_ne_nil (e : ExprStructure .char) :
+    e.elements ≠ [] := by
+  cases e <;> simp [elements]
+
+@[local simp]
+theorem ExprStructure.isEmpty_iff_elements_eq_nil (e : ExprStructure ty) :
+    e.isEmpty ↔ e.elements = [] := by
+  fun_induction isEmpty <;> simp_all [elements]
+
+inductive Path : ExprType → Type where
+  | root : Path .string
+  | stringAppendLeft (parent : Path .string) (right : ExprStructure .string) : Path .string
+  | stringAppendRight (parent : Path .string) (left : ExprStructure .string) : Path .string
+  | push (parent : Path .string) (c : ExprStructure .char) : Path .string
+  | toList (parent : Path .list) : Path .string
+
+  | cons (parent : Path .list) (c : ExprStructure .char) : Path .list
+  | listAppendLeft (parent : Path .list) (right : ExprStructure .list) : Path .list
+  | listAppendRight (parent : Path .list) (left : ExprStructure .list) : Path .list
+  | ofList (parent : Path .string) : Path .list
+
+  | singletonChar (parent : Path .string) : Path .char
+  | pushChar (parent : Path .string) (s : ExprStructure .string) : Path .char
+  | consChar (parent : Path .list) (l : ExprStructure .list) : Path .char
+  | litChar (parent : Path .string) (s : String.Slice) (p : s.str.Pos)
+    (h : p ≠ s.str.endPos) : Path .char
+deriving Repr
+
+def ExprStructure.litChar (s : String.Slice) (p : s.str.Pos) (h : p ≠ s.str.endPos) :
+    ExprStructure .char :=
+  if s.startInclusive ≤ p ∧ p < s.endExclusive then
+    .charLit (p.get h)
+  else
+    .erasedChar (mkCharLit (p.get h).toNat)
+
+@[local simp]
+theorem ExprStructure.elements_litChar (s : String.Slice) (p : s.str.Pos) (h : p ≠ s.str.endPos) :
+    (litChar s p h).elements = [.char (mkCharLit (p.get h).toNat)] := by
+  fun_cases litChar <;> simp [elements]
+
+@[unbox]
+structure Traverser where
+  {type : ExprType}
+  path : Path type
+  expr : ExprStructure type
+  of_eq_litChar (pa s p h) (h' : type = .char) :
+    h' ▸ path = .litChar pa s p h → expr = h' ▸ .litChar s p h
+deriving Repr
+
+def Traverser.root (e : ExprStructure .string) : Traverser := ⟨.root, e, nofun⟩
+
+def Path.toStruct : Path ty → ExprStructure ty → ExprStructure .string
+  | .root, e => e
+  -- String
+  | .stringAppendLeft parent right, left => parent.toStruct (.stringAppend left right)
+  | .stringAppendRight parent left, right => parent.toStruct (.stringAppend left right)
+  | .push parent c, s => parent.toStruct (.push s c)
+  | .toList parent, s => parent.toStruct (.toList s)
+  -- List Char
+  | .cons parent c, l => parent.toStruct (.cons c l)
+  | .listAppendLeft parent right, left => parent.toStruct (.listAppend left right)
+  | .listAppendRight parent left, right => parent.toStruct (.listAppend left right)
+  | .ofList parent, l => parent.toStruct (.ofList l)
+  -- Char
+  | .singletonChar parent, c => parent.toStruct (.singleton c)
+  | .pushChar parent s, c => parent.toStruct (.push s c)
+  | .consChar parent l, c => parent.toStruct (.cons c l)
+  | .litChar parent s _ _, _ => parent.toStruct (.stringLit s)
+
+def Path.prefix : Path ty → List Element
+  | .root => []
+  -- String
+  | .stringAppendLeft parent _ => parent.prefix
+  | .stringAppendRight parent left => parent.prefix ++ left.elements
+  | .push parent _ => parent.prefix
+  | .toList parent => parent.prefix
+  -- List Char
+  | .cons parent c => parent.prefix ++ c.elements
+  | .listAppendLeft parent _ => parent.prefix
+  | .listAppendRight parent left => parent.prefix ++ left.elements
+  | .ofList parent => parent.prefix
+  -- Char
+  | .singletonChar parent => parent.prefix
+  | .pushChar parent s => parent.prefix ++ s.elements
+  | .consChar parent _ => parent.prefix
+  | .litChar parent s p _ =>
+    parent.prefix ++ (s.str.sliceTo p).copy.toList.map (.char <| mkCharLit ·.toNat)
+
+def Path.suffix : Path ty → List Element
+  | .root => []
+  -- String
+  | .stringAppendLeft parent right => right.elements ++ parent.suffix
+  | .stringAppendRight parent _ => parent.suffix
+  | .push parent c => c.elements ++ parent.suffix
+  | .toList parent => parent.suffix
+  -- List Char
+  | .cons parent _ => parent.suffix
+  | .listAppendLeft parent right => right.elements ++ parent.suffix
+  | .listAppendRight parent _ => parent.suffix
+  | .ofList parent => parent.suffix
+  -- Char
+  | .singletonChar parent => parent.suffix
+  | .pushChar parent _ => parent.suffix
+  | .consChar parent l => l.elements ++ parent.suffix
+  | .litChar parent s p h =>
+    (s.str.sliceFrom (p.next h)).copy.toList.map (.char <| mkCharLit ·.toNat) ++ parent.suffix
+
+theorem Path.elements_toStruct (t : Traverser) :
+    (t.path.toStruct t.expr).elements = t.path.prefix ++ (t.expr.elements ++ t.path.suffix) := by
+  rcases t with ⟨path, expr, h⟩; dsimp only
+  fun_induction toStruct with (try simp [Path.prefix, Path.suffix, ExprStructure.elements, *]; done)
+  | case13 parent s p hp expr ih =>
+    specialize h parent s p hp rfl rfl
+    simp only [ne_eq, reduceCtorEq, forall_false, implies_true, ih, h]
+    simp [ExprStructure.elements, Path.prefix, Path.suffix]
+    conv => lhs; rw [String.Pos.eq_copy_sliceTo_append_get hp]
+    simp
+
+def Traverser.visitLeft : Traverser → Option Traverser
+  | ⟨p, .stringAppend l r, _⟩ =>
+    if l.isEmpty then
+      some ⟨.stringAppendRight p l, r, nofun⟩
+    else
+      some ⟨.stringAppendLeft p r, l, nofun⟩
+  | ⟨p, .push s c, _⟩ =>
+    if s.isEmpty then
+      some ⟨.pushChar p s, c, nofun⟩
+    else
+      some ⟨.push p c, s, nofun⟩
+  | ⟨p, .ofList l, _⟩ => some ⟨.ofList p, l, nofun⟩
+  | ⟨p, .singleton c, _⟩ => some ⟨.singletonChar p, c, nofun⟩
+  | ⟨p, .stringLit s, _⟩ =>
+    if h : s.str.isEmpty then
+      none
+    else
+      have h : s.str.startPos ≠ s.str.endPos := by simpa using h
+      some ⟨.litChar p s s.str.startPos h, .litChar _ _ h, by rintro _ _ _ _ _ ⟨⟩; rfl⟩
+  | ⟨p, .cons c l, _⟩ => some ⟨.consChar p l, c, nofun⟩
+  | ⟨p, .listAppend l r, _⟩ =>
+    if l.isEmpty then
+      some ⟨.listAppendRight p l, r, nofun⟩
+    else
+      some ⟨.listAppendLeft p r, l, nofun⟩
+  | ⟨p, .toList s, _⟩ => some ⟨.toList p, s, nofun⟩
+  | ⟨p, .anyString _, _⟩ => none
+  | ⟨p, .erasedString _, _⟩ => none
+  | ⟨p, .nil, _⟩ => none
+  | ⟨p, .anyList l, _⟩ => none
+  | ⟨p, .erasedList _, _⟩ => none
+  | ⟨p, .charLit c, _⟩ => none
+  | ⟨p, .anyChar c, _⟩ => none
+  | ⟨p, .erasedChar c, _⟩ => none
+
+theorem Traverser.toStruct_of_visitLeft_eq_some {t t' : Traverser}
+    (h : t.visitLeft = some t') : t.path.toStruct t.expr = t'.path.toStruct t'.expr := by
+  revert h; fun_cases visitLeft <;> rintro ⟨⟩ <;> simp [Path.toStruct]
+
+theorem Traverser.prefix_visitLeft_eq {t t' : Traverser}
+    (h : t.visitLeft = some t') : t'.path.prefix = t.path.prefix := by
+  revert h; fun_cases visitLeft <;> rintro ⟨⟩ <;> simp_all [Path.prefix]
+
+def Traverser.visitRight : Traverser → Option Traverser
+  | ⟨p, .stringAppend l r, _⟩ =>
+    if r.isEmpty then
+      some ⟨.stringAppendLeft p r, l, nofun⟩
+    else
+      some ⟨.stringAppendRight p l, r, nofun⟩
+  | ⟨p, .push s c, _⟩ => some ⟨.pushChar p s, c, nofun⟩
+  | ⟨p, .ofList l, _⟩ => some ⟨.ofList p, l, nofun⟩
+  | ⟨p, .singleton c, _⟩ => some ⟨.singletonChar p, c, nofun⟩
+  | ⟨p, .stringLit s, _⟩ =>
+    if h : s.str.isEmpty then
+      none
+    else
+      have h : s.str.endPos ≠ s.str.startPos := by rw [ne_comm]; simpa using h
+      have h' : s.str.endPos.prev h ≠ s.str.endPos := by simp
+      some ⟨.litChar p s _ h', .litChar _ _ h', by rintro _ _ _ _ _ ⟨⟩; rfl⟩
+  | ⟨p, .cons c l, _⟩ =>
+    if l.isEmpty then
+      some ⟨.consChar p l, c, nofun⟩
+    else
+      some ⟨.cons p c, l, nofun⟩
+  | ⟨p, .listAppend l r, _⟩ =>
+    if r.isEmpty then
+      some ⟨.listAppendLeft p r, l, nofun⟩
+    else
+      some ⟨.listAppendRight p l, r, nofun⟩
+  | ⟨p, .toList s, _⟩ => some ⟨.toList p, s, nofun⟩
+  | ⟨p, .anyString _, _⟩ => none
+  | ⟨p, .erasedString _, _⟩ => none
+  | ⟨p, .nil, _⟩ => none
+  | ⟨p, .anyList l, _⟩ => none
+  | ⟨p, .erasedList _, _⟩ => none
+  | ⟨p, .charLit c, _⟩ => none
+  | ⟨p, .anyChar c, _⟩ => none
+  | ⟨p, .erasedChar c, _⟩ => none
+
+theorem Traverser.toStruct_of_visitRight_eq_some {t t' : Traverser}
+    (h : t.visitRight = some t') : t.path.toStruct t.expr = t'.path.toStruct t'.expr := by
+  revert h; fun_cases visitRight <;> rintro ⟨⟩ <;> simp [Path.toStruct]
+
+theorem Traverser.suffix_visitRight_eq {t t' : Traverser}
+    (h : t.visitRight = some t') : t'.path.suffix = t.path.suffix := by
+  revert h; fun_cases visitRight <;> rintro ⟨⟩ <;> simp_all [Path.suffix]
+
+def Path.nextLeft : Path ty → ExprStructure ty → Traverser ⊕ ExprStructure .string
+  | .root, e => .inr e
+  -- String
+  | .stringAppendLeft parent right, left =>
+    if right.isEmpty then
+      parent.nextLeft (.stringAppend left right)
+    else
+      .inl ⟨.stringAppendRight parent left, right, nofun⟩
+  | .stringAppendRight parent left, right =>
+    parent.nextLeft (.stringAppend left right)
+  | .push parent c, s => .inl ⟨.pushChar parent s, c, nofun⟩
+  | .toList parent, s => parent.nextLeft (.toList s)
+  -- List Char
+  | .cons parent c, l => parent.nextLeft (.cons c l)
+  | .listAppendLeft parent right, left =>
+    if right.isEmpty then
+      parent.nextLeft (.listAppend left right)
+    else
+      .inl ⟨.listAppendRight parent left, right, nofun⟩
+  | .listAppendRight parent left, right =>
+    parent.nextLeft (.listAppend left right)
+  | .ofList parent, l => parent.nextLeft (.ofList l)
+  -- Char
+  | .singletonChar parent, c => parent.nextLeft (.singleton c)
+  | .pushChar parent s, c => parent.nextLeft (.push s c)
+  | .consChar parent l, c =>
+    if l.isEmpty then
+      parent.nextLeft (.cons c l)
+    else
+      .inl ⟨.cons parent c, l, nofun⟩
+  | .litChar parent s p h, _ =>
+    let s := { s with
+      startInclusive := if p.next h ≤ s.endExclusive then p.next h else s.startInclusive,
+      startInclusive_le_endExclusive := by split <;> simp [*, s.startInclusive_le_endExclusive] }
+    if h'' : p.next h = s.str.endPos then
+      parent.nextLeft (.stringLit s)
+    else
+      .inl ⟨.litChar parent s (p.next h) h'', .litChar s (p.next h) h'', by rintro _ _ _ _ _ ⟨⟩; rfl⟩
+
+theorem Path.nextLeft_matches_inl_iff {p : Path ty} {e : ExprStructure ty} :
+    p.nextLeft e matches .inl _ ↔ p.suffix ≠ [] := by
+  fun_induction nextLeft <;> simp_all +zetaDelta [suffix]
+
+theorem Path.prefix_nextLeft {t t' : Traverser} (h' : t.path.nextLeft t.expr = .inl t') :
+    t'.path.prefix = t.path.prefix ++ t.expr.elements := by
+  rcases t with ⟨path, expr, h⟩; revert h'; dsimp only
+  fun_induction nextLeft with
+    (try (first | rintro ⟨⟩ | intro) <;> simp_all [Path.prefix, ExprStructure.elements]; done)
+  | case16 parent s p hp s' hp' c ih =>
+    cases h _ _ _ _ rfl rfl; clear h
+    intro h'; rw [ih nofun h']; clear ih h'
+    simp only [ExprStructure.elements, Path.prefix, List.append_assoc, List.append_cancel_left_eq]
+    conv => lhs; rw [String.Pos.eq_copy_sliceTo_append_get hp, hp']
+    simp [s']
+  | case17 parent s p hp s' hp' c =>
+    cases h _ _ _ _ rfl rfl; clear h
+    rintro ⟨⟩; dsimp only
+    simp only [Path.prefix, ExprStructure.elements_litChar, List.append_assoc,
+      List.append_cancel_left_eq]
+    have : (s.str.sliceTo (p.next hp)).copy = (s.str.sliceTo p).copy ++ String.singleton (p.get hp) := by
+      rw [sliceTo_copy_eq_iff_exists_splits]
+      exact ⟨_, p.splits_next hp⟩
+    simp [s', this]
+
+theorem Path.suffix_nextLeft {t t' : Traverser} (h' : t.path.nextLeft t.expr = .inl t') :
+    t'.expr.elements ++ t'.path.suffix = t.path.suffix := by
+  rcases t with ⟨path, expr, h⟩; revert h'; dsimp only
+  fun_induction nextLeft with
+    (try (first | rintro ⟨⟩ | intro) <;> simp_all +zetaDelta [Path.suffix]; done)
+  | case17 parent s p hp s' hp' c =>
+    cases h _ _ _ _ rfl rfl; clear h
+    rintro ⟨⟩; dsimp only
+    simp only [ExprStructure.elements_litChar, suffix, List.cons_append, List.nil_append]
+    have : (s.str.sliceFrom (p.next hp)).copy =
+        String.singleton ((p.next hp).get hp') ++ (s.str.sliceFrom ((p.next hp).next hp')).copy := by
+      apply Pos.Splits.copy_sliceFrom_eq
+      exact (p.next hp).splits_next_right hp'
+    simp [s', this]
+
+def Path.nextRight : Path ty → ExprStructure ty → Traverser ⊕ ExprStructure .string
+  | .root, e => .inr e
+  -- String
+  | .stringAppendLeft parent right, left =>
+    parent.nextRight (.stringAppend left right)
+  | .stringAppendRight parent left, right =>
+    if left.isEmpty then
+      parent.nextRight (.stringAppend left right)
+    else
+      .inl ⟨.stringAppendLeft parent right, left, nofun⟩
+  | .push parent c, s => parent.nextRight (.push s c)
+  | .toList parent, s => parent.nextRight (.toList s)
+  -- List Char
+  | .cons parent c, l => .inl ⟨.consChar parent l, c, nofun⟩
+  | .listAppendLeft parent right, left =>
+    parent.nextRight (.listAppend left right)
+  | .listAppendRight parent left, right =>
+    if left.isEmpty then
+      parent.nextRight (.listAppend left right)
+    else
+      .inl ⟨.listAppendLeft parent right, left, nofun⟩
+  | .ofList parent, l => parent.nextRight (.ofList l)
+  -- Char
+  | .singletonChar parent, c => parent.nextRight (.singleton c)
+  | .pushChar parent s, c =>
+    if s.isEmpty then
+      parent.nextRight (.push s c)
+    else
+      .inl ⟨.push parent c, s, nofun⟩
+  | .consChar parent l, c => parent.nextRight (.cons c l)
+  | .litChar parent s p _, _ =>
+    let s := { s with
+      endExclusive := if s.startInclusive ≤ p then p else s.endExclusive,
+      startInclusive_le_endExclusive := by split <;> simp [*, s.startInclusive_le_endExclusive] }
+    if h : p = s.str.startPos then
+      parent.nextRight (.stringLit s)
+    else
+      .inl ⟨.litChar parent s (p.prev h) (by simp +zetaDelta),
+        .litChar s (p.prev h) (by simp +zetaDelta), by rintro _ _ _ _ _ ⟨⟩; rfl⟩
+
+theorem Path.nextRight_matches_inl_iff {p : Path ty} {e : ExprStructure ty} :
+    p.nextRight e matches .inl _ ↔ p.prefix ≠ [] := by
+  fun_induction nextRight <;> simp_all +zetaDelta [Path.prefix]
+
+theorem Path.suffix_nextRight {t t' : Traverser} (h' : t.path.nextRight t.expr = .inl t') :
+    t'.path.suffix = t.expr.elements ++ t.path.suffix := by
+  rcases t with ⟨path, expr, h⟩; revert h'; dsimp only
+  fun_induction nextRight with
+    (try (first | rintro ⟨⟩ | intro) <;> simp_all [Path.suffix, ExprStructure.elements]; done)
+  | case16 parent s p hp s' hp' c ih =>
+    cases h _ _ _ _ rfl rfl; clear h
+    intro h'; rw [ih nofun h']; clear ih h'
+    simp only [ExprStructure.elements, ExprStructure.elements_litChar, suffix, List.cons_append,
+      List.nil_append]
+    conv => lhs; rw [String.Pos.eq_copy_sliceTo_append_get hp]
+    simp [← hp', s']
+  | case17 parent s p hp hp' c =>
+    cases h _ _ _ _ rfl rfl; clear h
+    rintro ⟨⟩; dsimp only
+    simp only [suffix, ExprStructure.elements_litChar, List.cons_append, List.nil_append]
+    have : (s.str.sliceFrom p).copy = String.singleton (p.get hp) ++ (s.str.sliceFrom (p.next hp)).copy := by
+      apply Pos.Splits.copy_sliceFrom_eq
+      exact p.splits_next_right hp
+    simp +zetaDelta [this]
+
+theorem Path.prefix_nextRight {t t' : Traverser} (h' : t.path.nextRight t.expr = .inl t') :
+    t'.path.prefix ++ t'.expr.elements = t.path.prefix := by
+  rcases t with ⟨path, expr, h⟩; revert h'; dsimp only
+  fun_induction nextRight with
+    (try (first | rintro ⟨⟩ | intro) <;> simp_all +zetaDelta [Path.prefix]; done)
+  | case17 parent s p hp s' hp' c =>
+    cases h _ _ _ _ rfl rfl; clear h
+    rintro ⟨⟩; dsimp only
+    simp only [Path.prefix, ExprStructure.elements_litChar, List.append_assoc,
+      List.append_cancel_left_eq]
+    have : (s.str.sliceTo p).copy = (s.str.sliceTo (p.prev hp')).copy ++
+        String.singleton ((p.prev hp').get (by simp)) := by
+      apply Pos.Splits.copy_sliceTo_eq
+      exact p.splits_prev_right hp'
+    simp +zetaDelta [this]
+
+def obviousCharDiseq (a : ExprStructure ty) (b : ExprStructure ty') : Bool :=
+  match a, b with
+  | .charLit c, .charLit c' => c != c'
+  | _, _ => false
+
+def cancelLeft (a b : ExprStructure .string) :
+    MetaM (Array CancelElement × ExprStructure .string × ExprStructure .string) := do
+  if a.isEmpty || b.isEmpty then
+    return (#[], a, b)
+  let mut ta : Traverser := .root a
+  let mut tb : Traverser := .root b
+  let mut els : Array CancelElement := #[]
+  -- invariants:
+  -- `isDefEq (ta.path.toStruct ta.expr).toExpr a` and
+  -- `isDefEq (tb.path.toStruct tb.expr).toExpr b` and
+  -- `(els.map (·.left)).toList = ta.path.prefix` and
+  -- `(els.map (·.right)).toList = tb.path.prefix` and
+  -- `ta.expr.elements ≠ []` and `tb.expr.elements ≠ []`
+  repeat
+    if ← pure (ta.expr.maxDepth == tb.expr.maxDepth) then
+      if let some ⟨hty⟩ ← ta.expr.isCompatibleWith tb.expr then
+      let (aexpr, bexpr) : ExprStructure ta.type × ExprStructure tb.type ← match h : ta.type with
+        | .char =>
+          if ← ta.expr.isDefEq (hty ▸ tb.expr) then
+            els := els.push (.char ta.expr.toExpr)
+            pure (h ▸ .erasedChar ta.expr.toExpr, hty ▸ h ▸ .erasedChar ta.expr.toExpr)
+          else
+            els := els.push (.cons ta.expr.toExpr tb.expr.toExpr)
+            pure (h ▸ .erasedChar ta.expr.toExpr, hty ▸ h ▸ .erasedChar tb.expr.toExpr)
+        | .list =>
+          els := els.push (.list ta.expr.toExpr)
+          pure (h ▸ .erasedList ta.expr.toExpr, hty ▸ h ▸ .erasedList ta.expr.toExpr)
+        | .string =>
+          els := els.push (.string ta.expr.toExpr)
+          pure (h ▸ .erasedString ta.expr.toExpr, hty ▸ h ▸ .erasedString ta.expr.toExpr)
+      let ta' := ta.path.nextLeft aexpr
+      let tb' := tb.path.nextLeft bexpr
+      match ta', tb' with
+      | .inl ta', .inl tb' =>
+        if obviousCharDiseq ta.expr tb.expr then
+          return (els, ta.path.toStruct ta.expr, tb.path.toStruct tb.expr)
+        ta := ta'; tb := tb'
+        continue
+      | .inl ta', .inr b' => return (els, ta'.path.toStruct ta'.expr, b')
+      | .inr a', .inl tb' => return (els, a', tb'.path.toStruct tb'.expr)
+      | .inr a', .inr b' => return (els, a', b')
+    if ta.expr.maxDepth ≤ tb.expr.maxDepth then
+      if let some tb' := tb.visitLeft then
+        tb := tb'
+        continue
+    if tb.expr.maxDepth ≤ ta.expr.maxDepth then
+      if let some ta' := ta.visitLeft then
+        ta := ta'
+        continue
+    return (els, ta.path.toStruct ta.expr, tb.path.toStruct tb.expr)
+  unreachable!
+
+def cancelRight (a b : ExprStructure .string) :
+    MetaM (Array CancelElement × ExprStructure .string × ExprStructure .string) := do
+  if a.isEmpty || b.isEmpty then
+    return (#[], a, b)
+  let mut ta : Traverser := .root a
+  let mut tb : Traverser := .root b
+  let mut els : Array CancelElement := #[]
+  -- invariants:
+  -- `isDefEq (ta.path.toStruct ta.expr).toExpr a` and
+  -- `isDefEq (tb.path.toStruct tb.expr).toExpr b` and
+  -- `(els.map (·.left)).toList = ta.path.prefix` and
+  -- `(els.map (·.right)).toList = tb.path.prefix` and
+  -- `ta.expr.elements ≠ []` and `tb.expr.elements ≠ []`
+  repeat
+    if ← pure (ta.expr.maxDepth == tb.expr.maxDepth) then
+      if let some ⟨hty⟩ ← ta.expr.isCompatibleWith tb.expr then
+      let (aexpr, bexpr) : ExprStructure ta.type × ExprStructure tb.type ← match h : ta.type with
+        | .char =>
+          if ← ta.expr.isDefEq (hty ▸ tb.expr) then
+            els := els.push (.char ta.expr.toExpr)
+            pure (h ▸ .erasedChar ta.expr.toExpr, hty ▸ h ▸ .erasedChar ta.expr.toExpr)
+          else
+            els := els.push (.cons ta.expr.toExpr tb.expr.toExpr)
+            pure (h ▸ .erasedChar ta.expr.toExpr, hty ▸ h ▸ .erasedChar tb.expr.toExpr)
+        | .list =>
+          els := els.push (.list ta.expr.toExpr)
+          pure (h ▸ .erasedList ta.expr.toExpr, hty ▸ h ▸ .erasedList ta.expr.toExpr)
+        | .string =>
+          els := els.push (.string ta.expr.toExpr)
+          pure (h ▸ .erasedString ta.expr.toExpr, hty ▸ h ▸ .erasedString ta.expr.toExpr)
+      let ta' := ta.path.nextRight aexpr
+      let tb' := tb.path.nextRight bexpr
+      match ta', tb' with
+      | .inl ta', .inl tb' =>
+        if obviousCharDiseq ta.expr tb.expr then
+          return (els, ta.path.toStruct ta.expr, tb.path.toStruct tb.expr)
+        ta := ta'; tb := tb'
+        continue
+      | .inl ta', .inr b' => return (els, ta'.path.toStruct ta'.expr, b')
+      | .inr a', .inl tb' => return (els, a', tb'.path.toStruct tb'.expr)
+      | .inr a', .inr b' => return (els, a', b')
+    if ta.expr.maxDepth ≤ tb.expr.maxDepth then
+      if let some tb' := tb.visitRight then
+        tb := tb'
+        continue
+    if tb.expr.maxDepth ≤ ta.expr.maxDepth then
+      if let some ta' := ta.visitRight then
+        ta := ta'
+        continue
+    return (els, ta.path.toStruct ta.expr, tb.path.toStruct tb.expr)
+  unreachable!
+
+def abc : String := ""
+
+local elab "#test_cancel " l:term ", " r:term : command => do
+  Elab.Command.runTermElabM fun _ => do
+    let l ← Elab.Term.elabTermEnsuringType l (mkConst ``String)
+    let r ← Elab.Term.elabTermEnsuringType r (mkConst ``String)
+    Elab.Term.synthesizeSyntheticMVarsUsingDefault
+    withNewMCtxDepth do
+    withReducible do
+    let l ← createStringStructure l
+    let r ← createStringStructure r
+    logInfo l.toStructExpr
+    logInfo r.toStructExpr
+    let (els, l, r) ← cancelLeft l r
+    let (els', l, r) ← cancelRight l r
+    let l := l.removeErased.elim (.stringLit "") l
+    let r := r.removeErased.elim (.stringLit "") r
+    logInfo m!"Left cancel:{indentExpr (cancelElementToStruct els)}\n\
+               Right cancel:{indentExpr (cancelElementToStruct els'.reverse)}\n\
+               Left-hand side:{indentExpr l.toExpr}\n\
+               Right-hand side:{indentExpr r.toExpr}\n"
+
+variable (s : String) in
+#test_cancel "hi something something hd", "h".push 'i' ++ s ++ "hd"
+
+variable (s : String) (l : List Char) in
+#test_cancel (String.ofList ('a' :: 'b' :: l)).push 'b' ++ String.singleton 'a', "ab" ++ s ++ "ba"
+
+#eval withReducible <|
+  cancelLeft (.stringAppend (.stringLit "hi") (.anyString (.const ``abc []))) (.stringLit "hi there")
 
 public section
 
